Test/dafny0/DerivedTypes.dfy
@@ -44,3 +44,34 @@ method M()
     assert rounded == 6;
   }
 }
+
+module Constraints {
+  newtype SmallInt = x: int where 0 <= x < 100
+  newtype LargeInt = y: int where 0 <= y < 100
+
+  newtype A = x: int where 0 <= x
+  newtype B = x: A where x < 100
+  newtype C = B  // the constraints 0 <= x < 100 still apply
+
+  static predicate IsEven(x: int)  // note that this is a ghost predicate
+  {
+    x % 2 == 0
+  }
+  newtype G = x: int where IsEven(x)  // it's okay to use ghost constructs in type constraints
+
+  newtype N = nat
+
+  newtype AssertType = s: int where
+    var k := s;
+    assert k <= s;
+    k < 10 || 10 <= s
+
+  newtype Te = x: int where 0 <= x < 3 && [5, 7, 8][x] % 2 != 0
+
+  newtype Ta = x: int where 0 <= x < 3
+//  newtype Tb = y: Ta where [5, 7, 8][int(y)] % 2 != 0  // the indexing is okay, because of the type constraint for Ta
+
+  newtype Odds = x: int where x % 2 == 1  // error: cannot find witness
+
+  newtype K = x: real where 10.0 <= x ==> 200.0 / (x - 20.0) < 30.0  // error: division by zero
+}
